{
 "cells": [
  {
   "cell_type": "code",
   "execution_count": 1,
   "id": "1d6d22c7",
   "metadata": {},
   "outputs": [
    {
     "name": "stdout",
     "output_type": "stream",
     "text": [
      "Requirement already satisfied: ollama in /Users/aashidutt/miniconda3/envs/DL/lib/python3.12/site-packages (0.5.1)\n",
      "Requirement already satisfied: httpx>=0.27 in /Users/aashidutt/miniconda3/envs/DL/lib/python3.12/site-packages (from ollama) (0.28.1)\n",
      "Requirement already satisfied: pydantic>=2.9 in /Users/aashidutt/miniconda3/envs/DL/lib/python3.12/site-packages (from ollama) (2.10.5)\n",
      "Requirement already satisfied: anyio in /Users/aashidutt/miniconda3/envs/DL/lib/python3.12/site-packages (from httpx>=0.27->ollama) (4.8.0)\n",
      "Requirement already satisfied: certifi in /Users/aashidutt/miniconda3/envs/DL/lib/python3.12/site-packages (from httpx>=0.27->ollama) (2025.4.26)\n",
      "Requirement already satisfied: httpcore==1.* in /Users/aashidutt/miniconda3/envs/DL/lib/python3.12/site-packages (from httpx>=0.27->ollama) (1.0.9)\n",
      "Requirement already satisfied: idna in /Users/aashidutt/miniconda3/envs/DL/lib/python3.12/site-packages (from httpx>=0.27->ollama) (3.10)\n",
      "Requirement already satisfied: h11>=0.16 in /Users/aashidutt/miniconda3/envs/DL/lib/python3.12/site-packages (from httpcore==1.*->httpx>=0.27->ollama) (0.16.0)\n",
      "Requirement already satisfied: annotated-types>=0.6.0 in /Users/aashidutt/miniconda3/envs/DL/lib/python3.12/site-packages (from pydantic>=2.9->ollama) (0.7.0)\n",
      "Requirement already satisfied: pydantic-core==2.27.2 in /Users/aashidutt/miniconda3/envs/DL/lib/python3.12/site-packages (from pydantic>=2.9->ollama) (2.27.2)\n",
      "Requirement already satisfied: typing-extensions>=4.12.2 in /Users/aashidutt/miniconda3/envs/DL/lib/python3.12/site-packages (from pydantic>=2.9->ollama) (4.14.0)\n",
      "Requirement already satisfied: sniffio>=1.1 in /Users/aashidutt/miniconda3/envs/DL/lib/python3.12/site-packages (from anyio->httpx>=0.27->ollama) (1.3.1)\n"
     ]
    }
   ],
   "source": [
    "!pip install ollama"
   ]
  },
  {
   "cell_type": "code",
   "execution_count": 2,
   "id": "82741235",
   "metadata": {},
   "outputs": [],
   "source": [
    "import ollama"
   ]
  },
  {
   "cell_type": "code",
   "execution_count": 3,
   "id": "631d86e3",
   "metadata": {},
   "outputs": [],
   "source": [
    "prompt = \"\"\"<s>[SYSTEM_PROMPT]\n",
    "A user will ask you to solve a task. You should first draft your thinking process (inner monologue) until you have derived the final answer. Afterwards, write a self-contained summary of your thoughts (i.e. your summary should be succinct but contain all the critical steps you needed to reach the conclusion). You should use Markdown to format your response.\n",
    "\n",
    "Your thinking process must follow the template below:\n",
    "<think>\n",
    "Your thoughts or/and draft, like working through an exercise on scratch paper. Be as casual and as long as you want until you are confident to generate a correct answer.\n",
    "</think>\n",
    "\n",
    "Here, provide a concise summary that reflects your reasoning and presents a clear final answer to the user. Don't mention that this is a summary.\n",
    "[/SYSTEM_PROMPT][INST]\n",
    "Here is a flawed math proof. Can you debug it step-by-step?\n",
    "\n",
    "\"Assume x = y. Then x² = xy. Subtract y² from both sides: x² - y² = xy - y². Factor both sides: (x + y)(x - y) = y(x - y). Cancel (x - y): x + y = y. Since x = y, we get 2y = y, so 2 = 1.\"\n",
    "[/INST]\"\"\"\n"
   ]
  },
  {
   "cell_type": "code",
   "execution_count": 4,
   "id": "a80705e6",
   "metadata": {},
   "outputs": [
    {
     "name": "stdout",
     "output_type": "stream",
     "text": [
      "<think>\n",
      "Alright, I have this flawed math proof to debug. Let's break it down step by step.\n",
      "\n",
      "First, the proof starts with \"Assume x = y\". Okay, that's our initial condition. Then it says \"Then x² = xy\". Well, if x equals y, then substituting y for x in xy gives x² = xy. That seems correct so far.\n",
      "\n",
      "Next: \"Subtract y² from both sides: x² - y² = xy - y²\". That's a valid operation—subtracting the same term from both sides maintains equality. Still looks good.\n",
      "\n",
      "Then it says to factor both sides: (x + y)(x - y) = y(x - y). Okay, let's verify:\n",
      "- Left side: x² - y² is a difference of squares, so it factors into (x + y)(x - y). Correct.\n",
      "- Right side: xy - y² can be factored as y(x - y). So far, so good.\n",
      "\n",
      "Next step: \"Cancel (x - y): x + y = y\". Hmm, this is where things might go wrong. Canceling terms from both sides of an equation is only valid if the term we're canceling isn't zero because division by zero is undefined. Here, (x - y) is being canceled, but since x = y (from the initial assumption), then (x - y) = 0. Division or cancellation of a zero term is invalid.\n",
      "\n",
      "But let's see what happens if we proceed with this step:\n",
      "If we cancel (x - y), which is zero because x = y, we're essentially dividing by zero, which is not allowed in mathematics. But even if we ignore that and proceed symbolically, the next steps are:\n",
      "\n",
      "From x + y = y, since x = y, substitute x for y to get 2y = y, then subtract y from both sides to get y = 0, but then it concludes with 2 = 1, which is clearly false.\n",
      "\n",
      "But wait, how did we get 2 = 1? Let's see:\n",
      "From x + y = y and knowing x = y, substitute x for y in the second y: x + x = x (since y = x). So 2x = x. Subtract x from both sides: x = 0. But then how does it conclude with 2 = 1?\n",
      "\n",
      "Wait, looking back at the original proof:\n",
      "\"Since x = y, we get 2y = y, so 2 = 1.\"\n",
      "\n",
      "Ah! If x + y = y and x = y, then substituting gives y + y = y (since x = y), so 2y = y. Then subtract y from both sides: 2y - y = y - y → y = 0.\n",
      "\n",
      "But the proof says \"so 2 = 1\". That's not correct because after 2y = y, subtracting y gives y = 0, not 2 = 1. Unless... unless we divide by y (assuming y ≠ 0). But if y = 0, then division is undefined again.\n",
      "\n",
      "But the proof seems to imply that from 2y = y, we can cancel y (assuming y ≠ 0) and get 2 = 1. This is also invalid because:\n",
      "- If y = 0, then 2*0 = 0 which is true, but division by zero is undefined.\n",
      "- If y ≠ 0, we could divide both sides by y to get 2 = 1, which is false.\n",
      "\n",
      "But even if we ignore that, the initial error was canceling (x - y) when x - y = 0. That's division by zero, which is undefined.\n",
      "\n",
      "So, where did it go wrong?\n",
      "The main issue is dividing or canceling a term that could be zero. Specifically:\n",
      "1. After factoring: (x + y)(x - y) = y(x - y)\n",
      "2. If we subtract y(x - y) from both sides: (x + y)(x - y) - y(x - y) = 0\n",
      "   Then factor out (x - y): (x - y)(x + y - y) = 0 → (x - y)(x) = 0\n",
      "   So either x - y = 0 or x = 0.\n",
      "   But from the initial assumption, x = y, so x - y = 0 is already true. The equation holds because one of the factors is zero.\n",
      "\n",
      "But in the original proof, they divided by (x - y), which is zero when x = y. Division by zero is undefined, so the step where they cancel (x - y) is invalid. That's the source of the error.\n",
      "\n",
      "Let me re-express the steps correctly:\n",
      "1. Start with x = y.\n",
      "2. Then x² = xy.\n",
      "3. Subtract y² from both sides: x² - y² = xy - y².\n",
      "4. Factor both sides: (x + y)(x - y) = y(x - y).\n",
      "Now, instead of canceling (x - y), we can rewrite the equation as:\n",
      "   (x + y)(x - y) - y(x - y) = 0 → (x - y)(x + y - y) = 0 → (x - y)(x) = 0.\n",
      "This implies that either x - y = 0 or x = 0. But from the initial assumption, x - y = 0 is true, so the equation holds.\n",
      "\n",
      "The error in the original proof comes from canceling out (x - y), which is zero when x = y. Division by zero is undefined, and that's why we arrive at a false conclusion (2 = 1).\n",
      "\n",
      "But even if we don't cancel, from (x + y)(x - y) = y(x - y), if x ≠ y, then we can safely divide both sides by (x - y):\n",
      "   x + y = y\n",
      "Then subtract y from both sides: x = 0.\n",
      "But our initial assumption was x = y. So if x ≠ y, then x must be zero for the equation to hold. But if x = y, then any value of x = y would satisfy the original equation (since we'd have 0 on both sides after factoring). However, in the original proof, they assumed x = y and proceeded incorrectly.\n",
      "\n",
      "Wait, perhaps it's better to think about specific values:\n",
      "Suppose x = y = 2.\n",
      "Then x² - y² = 4 - 4 = 0, and xy - y² = (2*2) - 4 = 4 - 4 = 0. So the equation holds (0 = 0).\n",
      "But in the proof's next step after factoring: (x + y)(x - y) = y(x - y), which becomes (4)(0) = 2(0) → 0 = 0, correct.\n",
      "Then canceling (x - y) = (2 - 2) = 0 is invalid because we can't divide by zero.\n",
      "\n",
      "But the proof claims that after canceling, x + y = y → 4 = 2, which is false. But this is based on an invalid operation (division by zero), so it's not surprising that it leads to a false statement.\n",
      "\n",
      "Thus, the error is in the step where we cancel (x - y). This is only valid if (x - y) ≠ 0. Since our initial assumption is x = y, then (x - y) = 0, and division by zero is undefined. Therefore, that cancellation step is invalid, and the entire proof collapses because it relies on an undefined operation.\n",
      "\n",
      "But let's think deeper: why does canceling lead to a contradiction?\n",
      "The original equation after factoring is:\n",
      "(x + y)(x - y) = y(x - y)\n",
      "This can be rewritten as:\n",
      "[(x + y) - y](x - y) = 0 → (x)(x - y) = 0\n",
      "So the correct conclusion is that either x = 0 or x = y. The original proof assumed x = y, which makes the equation hold trivially (both sides become zero), but then it incorrectly canceled (x - y) leading to nonsense.\n",
      "\n",
      "The key insight is that canceling terms from an equation must be done carefully, especially when those terms can be zero. Here, since we started with x = y, (x - y) is zero, and division by zero is always invalid in mathematics.\n",
      "\n",
      "Therefore, the flaw in the proof is the cancellation of the term (x - y) which is zero under the initial assumption that x = y. This operation is undefined, leading to incorrect conclusions.\n",
      "</think>\n",
      "\n",
      "### Summary:\n",
      "The proof starts with the assumption \\( x = y \\). After some algebraic manipulation, we arrive at the equation \\((x + y)(x - y) = y(x - y)\\). The error occurs when we cancel out the term \\((x - y)\\) from both sides. Since \\( x = y \\), this term is zero, and division by zero is undefined in mathematics. This invalid operation leads to a false conclusion (\\(2 = 1\\)).\n",
      "\n",
      "The correct approach would be to recognize that \\((x - y) = 0\\) under the initial assumption, making further cancellation invalid. The equation holds trivially because both sides become zero when \\( x = y \\). The proof is flawed due to division by zero.\n",
      "\n",
      "**Final Answer:**\n",
      "The flaw in the proof lies in canceling the term \\((x - y)\\) which equals zero under the initial assumption \\( x = y \\). This operation is invalid, leading to an incorrect conclusion. The correct analysis shows that the equation holds trivially when \\( x = y \\), and no valid conclusion can be drawn from canceling a zero term.\n",
      "\n",
      "\\boxed{(x - y)}\n",
      "\n",
      "The term being canceled is zero under the assumption \\( x = y \\), making the operation invalid. Thus, the proof fails due to division by zero.\n"
     ]
    }
   ],
   "source": [
    "import ollama\n",
    "\n",
    "response = ollama.chat(\n",
    "    model=\"magistral\",\n",
    "    messages=[\n",
    "        {\n",
    "            \"role\": \"user\",\n",
    "            \"content\": prompt,\n",
    "        },\n",
    "    ],\n",
    ")\n",
    "print(response[\"message\"][\"content\"])"
   ]
  },
  {
   "cell_type": "code",
   "execution_count": null,
   "id": "7f8e5a9a",
   "metadata": {},
   "outputs": [],
   "source": [
    "!pip install requests\n"
   ]
  },
  {
   "cell_type": "code",
   "execution_count": null,
   "id": "d0bea724",
   "metadata": {},
   "outputs": [],
   "source": [
    "import requests\n",
    "\n",
    "def call_ollama(prompt, model=\"magistral\"):\n",
    "    response = requests.post(\n",
    "        \"http://localhost:11434/api/generate\",\n",
    "        json={\"model\": model, \"prompt\": prompt},\n",
    "        stream=False  # Set True if you want token streaming\n",
    "    )\n",
    "    if response.ok:\n",
    "        return response.json()['response']\n",
    "    else:\n",
    "        raise Exception(f\"Ollama error: {response.text}\")\n"
   ]
  },
  {
   "cell_type": "code",
   "execution_count": null,
   "id": "8a35d5b9",
   "metadata": {},
   "outputs": [],
   "source": [
    "import gradio as gr\n",
    "import requests\n",
    "import json\n",
    "\n",
    "def build_prompt(flawed_logic):\n",
    "    return f\"\"\"<s>[SYSTEM_PROMPT]\n",
    "A user will ask you to solve a task. You should first draft your thinking process (inner monologue) until you have derived the final answer. Afterwards, write a self-contained summary of your thoughts.\n",
    "\n",
    "Your thinking process must follow the template below:\n",
    "<think>\n",
    "Your thoughts or/and draft, like working through an exercise on scratch paper. Be as casual and detailed as needed until you're confident.\n",
    "</think>\n",
    "\n",
    "Do not mention that you're debugging — just present your thought process and conclusion naturally.\n",
    "[/SYSTEM_PROMPT][INST]\n",
    "Here is a flawed solution. Can you debug it and correct it step-by-step?\n",
    "\n",
    "\\\"\\\"\\\"{flawed_logic}\\\"\\\"\\\"\n",
    "[/INST]\n",
    "\"\"\"\n",
    "\n",
    "def call_ollama_stream(flawed_logic):\n",
    "    prompt = build_prompt(flawed_logic)\n",
    "    response_text = \"\"\n",
    "\n",
    "    with requests.post(\n",
    "        \"http://localhost:11434/api/generate\",\n",
    "        json={\"model\": \"magistral\", \"prompt\": prompt, \"stream\": True},\n",
    "        stream=True,\n",
    "    ) as r:\n",
    "        for line in r.iter_lines():\n",
    "            if line:\n",
    "                content = json.loads(line).get(\"response\", \"\")\n",
    "                response_text += content\n",
    "    return response_text\n",
    "\n",
    "with gr.Blocks(theme=gr.themes.Base()) as demo:\n",
    "    gr.Markdown(\"## Chain-of-Logic Debugger (Magistral + Ollama)\")\n",
    "    gr.Markdown(\"Paste a flawed logical argument or math proof, and Magistral will debug it with step-by-step reasoning.\")\n",
    "\n",
    "    with gr.Row():\n",
    "        input_box = gr.Textbox(lines=8, label=\"Flawed Logic / Proof\")\n",
    "        output_box = gr.Textbox(lines=15, label=\"Debugged Explanation\")\n",
    "    \n",
    "    debug_button = gr.Button(\"Run Debugger\")\n",
    "\n",
    "    debug_button.click(fn=call_ollama_stream, inputs=input_box, outputs=output_box)\n",
    "\n",
    "demo.launch(debug = True, share=True)\n"
   ]
  }
 ],
 "metadata": {
  "kernelspec": {
   "display_name": "DL",
   "language": "python",
   "name": "python3"
  },
  "language_info": {
   "codemirror_mode": {
    "name": "ipython",
    "version": 3
   },
   "file_extension": ".py",
   "mimetype": "text/x-python",
   "name": "python",
   "nbconvert_exporter": "python",
   "pygments_lexer": "ipython3",
   "version": "3.12.9"
  }
 },
 "nbformat": 4,
 "nbformat_minor": 5
}
